Auto/Lib/BinTree.lean
@@ -30,7 +30,7 @@ private theorem wfAux (n n' : Nat) : n = n' + 2 → n / 2 < n := by
   {motive : Nat → Sort u} (x : Nat)
   (ind : ∀ x, motive ((x + 2) / 2) → motive (x + 2))
   (base₀ : motive 0) (base₁ : motive 1) : motive x :=
-  match h : x with
+  match _h : x with
   | 0 => base₀
   | 1 => base₁
   | x' + 2 => ind x' (inductionOn ((x' + 2) / 2) ind base₀ base₁)
@@ -117,7 +117,7 @@ def right! (bt : BinTree α) :=
   | .node _ _ r => r
 
 def get?'WF (bt : BinTree α) (n : Nat) : Option α :=
-  match h : n with
+  match _h : n with
   | 0 => .none
   | 1 => bt.val?
   | _ + 2 =>
@@ -125,7 +125,7 @@ def get?'WF (bt : BinTree α) (n : Nat) : Option α :=
     | 0 => get?'WF bt.left! (Nat.div n 2)
     | _ + 1 => get?'WF bt.right! (Nat.div n 2)
 termination_by n
-decreasing_by all_goals { rw [← h]; apply Bin.wfAux; assumption }
+decreasing_by all_goals { rw [← _h]; apply Bin.wfAux; assumption }
 
 theorem get?'WF.succSucc (bt : BinTree α) (n : Nat) :
   get?'WF bt (n + 2) =
@@ -198,7 +198,7 @@ theorem get?'_leaf (n : Nat) : @get?' α .leaf n = .none := by
     cases (n + 2) % 2 <;> exact IH
 
 def insert'WF (bt : BinTree α) (n : Nat) (x : α) : BinTree α :=
-  match h : n with
+  match _h : n with
   | 0 => bt
   | 1 =>
     match bt with
@@ -215,7 +215,7 @@ def insert'WF (bt : BinTree α) (n : Nat) (x : α) : BinTree α :=
       | .leaf => .node .leaf .none (insert'WF .leaf (Nat.div n 2) x)
       | .node l v r => .node l v (insert'WF r (Nat.div n 2) x)
 termination_by n
-decreasing_by all_goals { rw [← h]; apply Bin.wfAux; assumption }
+decreasing_by all_goals { rw [← _h]; apply Bin.wfAux; assumption }
 
 theorem insert'WF.succSucc (bt : BinTree α) (n : Nat) (x : α) :
   insert'WF bt (n + 2) x =
